WIP adding strong leadership

isabelle/Implementation.thy
@@ -6,46 +6,135 @@ theory Implementation
   imports Preliminaries
 begin
 
+subsection \<open>Protocol messages\<close>
+
+text \<open>The
+proven-safe core of the protocol works by sending messages as described here. The remainder of the
+protocol may send other messages too, and may drop, reorder or duplicate any of these messages, but
+must not send these messages itself to ensure safety. Another way of thinking of these messages is
+to consider them as ``fire-and-forget'' RPC invocations that, on receipt, call some local method, maybe
+update the receiving node's state, and maybe yield some further messages. The @{type nat} parameter to each
+message refers to a slot number.\<close>
+
+
+datatype Message
+  = StartJoin Term
+  | JoinRequest nat Term "Term option"
+  | ClientValue Value
+  | PublishRequest nat Term Value
+  | PublishResponse nat Term
+  | ApplyCommit nat Term
+  | Reboot
+
+text \<open>Some prose descriptions of these messages follows, in order to give a bit more of an
+intuitive understanding of their purposes.\<close>
+
+text \<open>The message @{term "StartJoin t"} may be sent by any node to attempt to start a master
+election in the given term @{term t}.\<close>
+
+text \<open>The message @{term "JoinRequest i t a"} may be sent by a node in response
+to a @{term StartJoin} message. It indicates that the sender knows all committed values for slots
+strictly below @{term i}, and that the sender will no longer vote (i.e. send an @{term
+PublishResponse}) in any term prior to @{term t}. The field @{term a} is either @{term
+None} or @{term "Some t'"}. In the former case this indicates that
+the node has not yet sent any @{term PublishResponse} message in slot @{term i}, and in the latter
+case it indicates that the largest term in which it has previously sent an @{term PublishResponse}
+message is @{term t'}.  All
+nodes must avoid sending a @{term JoinRequest} message to two different masters in the same term.\<close>
+
+text \<open>The message @{term "ClientValue x"} may be sent by any node and indicates an attempt to
+reach consensus on the value @{term x}.\<close>
+
+text \<open>The message @{term "PublishRequest i t v"} may be sent by the elected master of term
+@{term t} to request the other master-eligible nodes to vote for value @{term v} to be committed in
+slot @{term i}.\<close>
+
+text \<open>The message @{term "PublishResponse i t"} may be sent by node in response to
+the corresponding @{term PublishRequest} message, indicating that the sender votes for the value
+proposed by the master of term @{term t} to be committed in slot @{term i}.\<close>
+
+text \<open>The message @{term "ApplyCommit i t"} indicates that the value proposed by the master of
+term @{term t} in slot @{term i} received a quorum of votes and is therefore committed.\<close>
+
+text \<open>The message @{term Reboot} may be sent by any node to represent the restart of a node, which
+loses any ephemeral state.\<close>
+
+text \<open>The abstract model of Zen keeps track of the set of all messages that have ever been
+sent, and asserts that this set obeys certain invariants, listed below. Further below, it will be
+shown that these invariants imply that each slot obeys the @{term oneSlot} invariants above and
+hence that each slot cannot see inconsistent committed values.\<close>
+
+datatype Destination = Broadcast | OneNode Node
+
+record RoutedMessage =
+  sender :: Node
+  destination :: Destination
+  payload :: Message
+
+text \<open>It will be useful to be able to choose the optional term with the greater term,
+so here is a function that does that.\<close>
+
+fun maxTermOption :: "Term option \<Rightarrow> Term option \<Rightarrow> Term option"
+  where
+    "maxTermOption None None = None"
+  | "maxTermOption None (Some t) = Some t"
+  | "maxTermOption (Some t) None = Some t"
+  | "maxTermOption (Some t\<^sub>1) (Some t\<^sub>2) = Some (max t\<^sub>1 t\<^sub>2)"
+
+lemma maxTermOption_t_None[simp]: "maxTermOption mt None = mt" by (cases mt, auto)
+lemma maxTermOption_None_t[simp]: "maxTermOption None mt = mt" by (cases mt, auto)
+
+lemma 
+  assumes "maxTermOption p1 p2 = None"
+  shows maxTermOption_eq_None_1:"p1 = None"
+    and maxTermOption_eq_None_2:"p2 = None"
+  using assms maxTermOption.elims by auto
+
+lemma maxTermOption_range: "maxTermOption p1 p2 \<in> {p1, p2}"
+  by (cases p1, simp, cases p2, simp_all add: max_def)
+
+subsection \<open>Node implementation\<close>
+
 text \<open>Each node holds the following local data.\<close>
+
+datatype ElectionValueState
+  = ElectionValueFree (* all received promises carried no previously-accepted term. Can propose anything. *)
+  | ElectionValueUnknown (* received a promise carrying a previously-accepted term, but it wasn't the local lastAcceptedTerm so it is unknown. Cannot propose anything. *)
+  | ElectionValueForced (* received a promise carrying a previously-accepted term equal to the local lastAcceptedTerm. Can propose the last-accepted value. *)
 
 record NodeData =
   currentNode :: Node (* identity of this node *)
   firstUncommittedSlot :: nat (* all slots strictly below this one are committed *)
+  currentTerm :: Term (* greatest term for which a promise was sent, and term of votes being collected *)
   currentEra :: Era (* era of the firstUncommittedSlot slot *)
   currentConfiguration :: Configuration (* configuration of the currentEra *)
   currentClusterState :: ClusterState (* last-committed cluster state *)
   (* acceptor data *)
-  lastAccepted :: PreviousPublishResponse (* term and value that were last accepted in this slot, if any *)
-  currentTerm :: Term (* greatest term for which a promise was sent, and term of votes being collected *)
+  lastAcceptedTerm :: "Term option" (* term that was last accepted in this slot, if any *)
+  lastAcceptedValue :: Value (* value accepted in lastAcceptedTerm, or NoOp *)
   (* election data *)
-  electionVotes :: "Node set" (* set of nodes that have sent a JoinRequest for the current currentTerm *)
+  joinVotes :: "Node set" (* set of nodes that have sent a JoinRequest for the current currentTerm *)
   electionWon :: bool
-  electionValue :: PreviousPublishResponse
+  electionValueState :: ElectionValueState (* if True, must propose lastAcceptedValue for this slot on winning an election; if False, can propose anything *)
   (* learner data *)
-  applyRequested :: bool (* whether an PublishRequest has been sent with slot=firstUncommittedSlot and term=currentTerm *)
-  applyVotes :: "Node set"
-
-definition lastAcceptedGreaterTermThan :: "Term \<Rightarrow> NodeData \<Rightarrow> bool"
-  where
-    "lastAcceptedGreaterTermThan t nd \<equiv> case lastAccepted nd of
-      NoPublishResponseSent \<Rightarrow> False
-      | PublishResponseSent t' _ \<Rightarrow> t' < t"
+  publishPermitted :: bool (* if True, may publish a value for this slot/term pair; if False, must not. *)
+  publishVotes :: "Node set"
 
 definition isQuorum :: "NodeData \<Rightarrow> Node set \<Rightarrow> bool"
   where "isQuorum nd q \<equiv> q \<in> Rep_Configuration (currentConfiguration nd)"
 
 text \<open>This method updates the node's state when a value is committed.\<close>
 
-definition applyValue :: "Value \<Rightarrow> NodeData \<Rightarrow> NodeData"
+definition applyAcceptedValue :: "NodeData \<Rightarrow> NodeData"
   where
-    "applyValue x nd \<equiv> case x of
+    "applyAcceptedValue nd \<equiv> case lastAcceptedValue nd of
         NoOp \<Rightarrow> nd
       | Reconfigure Q \<Rightarrow> nd
           \<lparr> currentEra := nextEra (currentEra nd)
           , currentConfiguration := Q
-          , electionVotes := {}
+          , joinVotes := {}
           , electionWon := False
-          , electionValue := NoPublishResponseSent \<rparr>
+          , electionValueState := ElectionValueFree \<rparr>
       | SetClusterState s \<Rightarrow> nd \<lparr> currentClusterState := s \<rparr>"
 
 text \<open>This method publishes a value via a @{term PublishRequest} message.\<close>
@@ -53,22 +142,12 @@ text \<open>This method publishes a value via a @{term PublishRequest} message.\
 definition publishValue :: "Value \<Rightarrow> NodeData \<Rightarrow> (NodeData * Message option)"
   where
     "publishValue x nd \<equiv>
-        if electionWon nd \<and> \<not> applyRequested nd
-              then ( nd \<lparr> applyRequested := True \<rparr>
+        if electionWon nd \<and> publishPermitted nd
+              then ( nd \<lparr> publishPermitted := False \<rparr>
                    , Some (PublishRequest
                              (firstUncommittedSlot nd)
                              (currentTerm nd) x) )
               else (nd, None)"
-
-text \<open>Some elections require the new master to retry a previous attempt at publication, which
-is what this method does.\<close>
-
-definition sendElectionValueIfAppropriate :: "NodeData \<Rightarrow> (NodeData * Message option)"
-  where
-    "sendElectionValueIfAppropriate nd
-      \<equiv> case electionValue nd of
-          PublishResponseSent _ x \<Rightarrow> publishValue x nd
-          | _ \<Rightarrow> (nd, None)"
 
 text \<open>This method updates the node's current term (if necessary) and discards any data associated
 with the previous term.\<close>
@@ -79,23 +158,26 @@ definition ensureCurrentTerm :: "Term \<Rightarrow> NodeData \<Rightarrow> NodeD
         if currentTerm nd = t
             then nd
             else nd
-              \<lparr> electionVotes := {}
+              \<lparr> joinVotes := {}
               , currentTerm := t
               , electionWon := False
-              , electionValue := NoPublishResponseSent
-              , applyRequested := False
-              , applyVotes := {} \<rparr>"
+              , electionValueState := ElectionValueFree
+              , publishPermitted := True
+              , publishVotes := {} \<rparr>"
 
 text \<open>This method updates the node's state on receipt of a vote (a @{term JoinRequest}) in an election.\<close>
 
-definition addElectionVote :: "Node \<Rightarrow> nat => PreviousPublishResponse \<Rightarrow> NodeData \<Rightarrow> NodeData"
+definition addElectionVote :: "Node \<Rightarrow> nat => Term option \<Rightarrow> NodeData \<Rightarrow> NodeData"
   where
-    "addElectionVote s i a nd \<equiv> let newVotes = insert s (electionVotes nd)
-      in nd \<lparr> electionVotes := newVotes
-            , electionValue := combinePublishResponses (electionValue nd)
-                                                     (if i = firstUncommittedSlot nd
-                                                        then a
-                                                        else NoPublishResponseSent)
+    "addElectionVote s i a nd \<equiv> let newVotes = insert s (joinVotes nd)
+      in nd \<lparr> joinVotes := newVotes
+            , electionValueState :=
+                if i = firstUncommittedSlot nd \<and> a \<noteq> None
+                then if a = lastAcceptedTerm nd
+                          \<or> electionValueState nd = ElectionValueForced
+                         then ElectionValueForced
+                         else ElectionValueUnknown
+                else electionValueState nd
             , electionWon := isQuorum nd newVotes \<rparr>"
 
 text \<open>Clients request the cluster to achieve consensus on certain values using the @{term ClientValue}
@@ -104,7 +186,7 @@ message which is handled as follows.\<close>
 definition handleClientValue :: "Value \<Rightarrow> NodeData \<Rightarrow> (NodeData * Message option)"
   where
     "handleClientValue x nd \<equiv>
-      if electionValue nd = NoPublishResponseSent
+      if electionValueState nd = ElectionValueFree
         then publishValue x nd
         else (nd, None)"
 
@@ -113,27 +195,30 @@ node's term and yielding a @{term JoinRequest} message as follows.\<close>
 
 definition handleStartJoin :: "Term \<Rightarrow> NodeData \<Rightarrow> (NodeData * Message option)"
   where
-    "handleStartJoin t nd \<equiv> if currentTerm nd < t \<and> era\<^sub>t t = currentEra nd
+    "handleStartJoin t nd \<equiv>
+        if currentTerm nd < t 
+             \<and> era\<^sub>t t = currentEra nd
           then ( ensureCurrentTerm t nd
                , Some (JoinRequest (firstUncommittedSlot nd)
                                      t
-                                    (lastAccepted nd)))
+                                    (lastAcceptedTerm nd)))
           else (nd, None)"
 
 text \<open>A @{term JoinRequest} message is checked for acceptability and then handled as follows, perhaps
 yielding a @{term PublishRequest} message.\<close>
 
-definition handleJoinRequest :: "Node \<Rightarrow> nat \<Rightarrow> Term \<Rightarrow> PreviousPublishResponse \<Rightarrow> NodeData \<Rightarrow> (NodeData * Message option)"
+definition handleJoinRequest :: "Node \<Rightarrow> nat \<Rightarrow> Term \<Rightarrow> Term option \<Rightarrow> NodeData \<Rightarrow> (NodeData * Message option)"
   where
     "handleJoinRequest s i t a nd \<equiv>
-         if firstUncommittedSlot nd < i
-             \<or> t < currentTerm nd
-             \<or> (t = currentTerm nd \<and> electionWon nd)
-             \<or> era\<^sub>t t \<noteq> currentEra nd
-          then (nd, None)
-          else let nd1 = ensureCurrentTerm t nd;
+         if i \<le> firstUncommittedSlot nd
+             \<and> era\<^sub>t t = currentEra nd
+             \<and> currentTerm nd \<le> t
+             \<and> (currentTerm nd = t \<longrightarrow> \<not> electionWon nd)
+             \<and> (maxTermOption a (lastAcceptedTerm nd) = lastAcceptedTerm nd) (* TODO \<or> i < firstUncommittedSlot *)
+          then let nd1 = ensureCurrentTerm t nd;
                    nd2 = addElectionVote s i a nd1
-               in sendElectionValueIfAppropriate nd2"
+               in publishValue (lastAcceptedValue nd2) nd2
+          else (nd, None)"
 
 text \<open>A @{term PublishRequest} message is checked for acceptability and then handled as follows,
 yielding a @{term PublishResponse} message.\<close>
@@ -141,10 +226,10 @@ yielding a @{term PublishResponse} message.\<close>
 definition handlePublishRequest :: "nat \<Rightarrow> Term \<Rightarrow> Value \<Rightarrow> NodeData \<Rightarrow> (NodeData * Message option)"
   where
     "handlePublishRequest i t x nd \<equiv>
-          if currentTerm nd \<le> t
-                \<and> \<not> lastAcceptedGreaterTermThan t nd
-                \<and> firstUncommittedSlot nd = i
-          then ( nd \<lparr> lastAccepted := PublishResponseSent t x \<rparr>
+          if i = firstUncommittedSlot nd
+                \<and> currentTerm nd \<le> t
+                \<and> (case lastAcceptedTerm nd of None \<Rightarrow> True | Some t' \<Rightarrow> t' \<le> t)
+          then ( nd \<lparr> lastAcceptedTerm := Some t, lastAcceptedValue := x \<rparr>
                , Some (PublishResponse i t))
           else (nd, None)"
 
@@ -155,10 +240,11 @@ value is committed, yielding an @{term ApplyCommit} message.\<close>
 definition handlePublishResponse :: "Node \<Rightarrow> nat \<Rightarrow> Term \<Rightarrow> NodeData \<Rightarrow> (NodeData * Message option)"
   where
     "handlePublishResponse s i t nd \<equiv>
-        if firstUncommittedSlot nd = i \<and> currentTerm nd \<le> t
+        if i = firstUncommittedSlot nd
+             \<and> currentTerm nd \<le> t
         then let nd1 = ensureCurrentTerm t nd;
-                 newVotes = insert s (applyVotes nd1)
-             in (nd1 \<lparr> applyVotes := newVotes \<rparr>,
+                 newVotes = insert s (publishVotes nd1)
+             in (nd1 \<lparr> publishVotes := newVotes \<rparr>,
                  if isQuorum nd newVotes then Some (ApplyCommit i t) else None)
         else (nd, None)"
 
@@ -169,17 +255,14 @@ definition handleApplyCommit :: "nat \<Rightarrow> Term \<Rightarrow> NodeData \
   where
     "handleApplyCommit i t nd \<equiv> 
         if i = firstUncommittedSlot nd
-        then case lastAccepted nd of
-            PublishResponseSent t' x' \<Rightarrow>
-              if t = t'
-              then applyValue x'
-                      nd \<lparr> firstUncommittedSlot := i + 1
-                         , lastAccepted := NoPublishResponseSent
-                         , applyRequested := False
-                         , electionValue := NoPublishResponseSent \<rparr>
-              else nd
-          | NoPublishResponseSent \<Rightarrow> nd
-        else nd"
+         \<and> lastAcceptedTerm nd = Some t
+          then applyAcceptedValue
+                  nd \<lparr> firstUncommittedSlot := i + 1
+                     , lastAcceptedValue := NoOp
+                     , lastAcceptedTerm := None
+                     , publishPermitted := True
+                     , electionValueState := ElectionValueFree \<rparr>
+          else nd"
 
 text \<open>A @{term Reboot} message simulates the effect of a reboot, discarding any ephemeral state but
 preserving the persistent state. It yields no messages.\<close>
@@ -189,16 +272,17 @@ definition handleReboot :: "NodeData \<Rightarrow> NodeData"
     "handleReboot nd \<equiv> 
       \<lparr> currentNode = currentNode nd
       , firstUncommittedSlot = firstUncommittedSlot nd
+      , currentTerm = currentTerm nd
       , currentEra = currentEra nd
       , currentConfiguration = currentConfiguration nd
       , currentClusterState = currentClusterState nd
-      , lastAccepted = lastAccepted nd
-      , currentTerm = currentTerm nd
-      , electionVotes = {}
+      , lastAcceptedTerm = lastAcceptedTerm nd
+      , lastAcceptedValue = lastAcceptedValue nd
+      , joinVotes = {}
       , electionWon = False
-      , electionValue = NoPublishResponseSent
-      , applyRequested = True
-      , applyVotes = {} \<rparr>"
+      , electionValueState = ElectionValueFree
+      , publishPermitted = False
+      , publishVotes = {} \<rparr>"
 
 text \<open>This function dispatches incoming messages to the appropriate handler method, and
 routes any responses to the appropriate places. In particular, @{term JoinRequest} messages
